slem/step.v
@@ -1,0 +1,293 @@
+From mathcomp Require Import ssreflect.seq all_ssreflect.
+From Paco Require Import paco pacotac.
+From SST Require Export src.expressions src.header src.global src.local src.merge src.global_tree_ctx src.projection src.step.
+Require Import List String Coq.Arith.PeanoNat Relations Coq.Logic.Decidable.
+Import ListNotations. 
+
+Lemma wfgC_step_part_helper : forall lis1 xs,
+    SList lis1 -> 
+    Forall2
+       (fun (u : option (sort * global)) (v : option (sort * gtt)) =>
+        u = None /\ v = None \/
+        (exists (s : sort) (g : global) (g' : gtt),
+           u = Some (s, g) /\ v = Some (s, g') /\ upaco2 gttT bot2 g g')) lis1 xs -> 
+    SList xs.
+Proof.
+  induction lis1; intros; try easy.
+  destruct xs; try easy.
+  specialize(SList_f a lis1 H); intros.
+  inversion H0. clear H0. subst.
+  destruct H1. apply SList_b. specialize(IHlis1 xs). apply IHlis1; try easy.
+  destruct H0. destruct H1. subst. destruct xs; try easy.
+  destruct H5; try easy. destruct H0 as (s0,(g0,(g1,(Ha,(Hb,Hc))))). inversion Ha. subst.
+  easy.
+Qed.
+
+Lemma wfgC_step_part : forall G G' p q n,
+    wfgC G ->
+    gttstepC G G' p q n -> 
+    isgPartsC p G.
+Proof.
+  intros.
+  - pinversion H0. subst. 
+    apply triv_pt_p; try easy.
+  - subst.
+    unfold wfgC in H.
+    destruct H as (Gl,(Ha,(Hb,(Hc,Hd)))). 
+    specialize(guard_breakG_s2 (gtt_send r s xs) Gl Hc Hb Ha); intros.
+    clear Ha Hb Hc. clear Gl. destruct H as (Gl,(Ha,(Hb,(Hc,He)))).
+    destruct Ha. subst. pinversion He. apply gttT_mon.
+    destruct H as (p1,(q1,(lis1,Ht))). subst. pinversion He. subst.
+    inversion Hc. subst.
+    specialize(wfgC_step_part_helper lis1 xs H12 H9); intros.
+    clear H14 H13.
+    unfold isgPartsC.
+    specialize(slist_implies_some xs H); intros. destruct H10 as (k,(G,Hta)).
+    specialize(some_onth_implies_In k xs G Hta); intros.
+    specialize(Forall_forall (fun u : option (sort * gtt) =>
+        u = None \/ (exists (s : sort) (g : gtt), u = Some (s, g) /\ isgPartsC p g /\ isgPartsC q g)) xs); intros.
+    destruct H11. specialize(H11 H7). clear H13 H7.
+    specialize(H11 (Some G) H10). destruct H11; try easy. 
+    destruct H7 as (s1,(g1,(Hsa,(Hsb,Hsc)))). inversion Hsa. subst.
+    unfold isgPartsC in Hsb. destruct Hsb as (G1,(Hla,(Hlb,Hlc))).
+    exists (g_send r s (overwrite_lis k (Some (s1, G1)) lis1)). 
+    clear Hsc H10 Hsa H H12 He H8. clear H6 H4 H2 H1 Hd H0 Hc.
+    revert Hlc Hlb Hla Hta H9 Hb H5 H3. revert G1 g1 s1 lis1 xs r s p. clear q n ys.
+    induction k; intros; try easy.
+    - destruct xs; try easy. destruct lis1; try easy. 
+      inversion H9. subst. clear H9.
+      simpl in Hta. subst.
+      destruct H2; try easy. destruct H as (s2,(g2,(g3,(Hsa,(Hsb,Hsc))))).
+      inversion Hsb. subst.
+      split.
+      - pfold. constructor. constructor; try easy.
+        right. exists s2. exists G1. exists g3. split. easy. split. easy. left. easy.
+      - split.
+        apply guard_cont_b.
+        specialize(guard_cont Hb); intros. inversion H. subst. clear H.
+        constructor; try easy. right. exists s2. exists G1. easy.
+      - apply pa_sendr with (n := 0) (s := s2) (g := G1); try easy.
+    - destruct xs; try easy. destruct lis1; try easy. 
+      inversion H9. subst. clear H9.
+      specialize(IHk G1 g1 s1 lis1 xs).
+      specialize(guard_cont Hb); intros. inversion H. subst. clear H.
+      assert((forall n : fin, exists m : fin, guardG n m (g_send r s lis1))). apply guard_cont_b; try easy.
+      assert(gttTC (g_send r s (overwrite_lis k (Some (s1, G1)) lis1)) (gtt_send r s xs) /\
+      (forall n : fin, exists m : fin, guardG n m (g_send r s (overwrite_lis k (Some (s1, G1)) lis1))) /\
+      isgParts p (g_send r s (overwrite_lis k (Some (s1, G1)) lis1))).
+      {
+        apply IHk; try easy.
+      }
+      destruct H0 as (Hma,(Hmb,Hmc)).
+      - split. pfold. constructor.
+        pinversion Hma; try easy. subst. constructor; try easy. apply gttT_mon.
+      - split. apply guard_cont_b; try easy. simpl.
+        specialize(guard_cont Hmb); intros.
+        constructor; try easy.
+      - apply pa_sendr with (n := S k) (s := s1) (g := G1); try easy.
+        apply overwriteExtract; try easy.
+      apply gttT_mon.
+      apply step_mon.
+Qed.
+
+
+Lemma part_after_step_helper2 : forall l x0 q p x G' pt s,
+    isgPartsC pt G' -> 
+    Some (s, G') = onth l x0 -> 
+    gttTC (g_send q p x) (gtt_send q p x0) -> 
+    (forall n : fin, exists m : fin, guardG n m (g_send q p x)) ->
+    exists G'0 : global, gttTC G'0 (gtt_send q p x0) /\ (forall n : fin, exists m : fin, guardG n m G'0) /\ isgParts pt G'0.
+Proof.  
+  intros.
+  unfold isgPartsC in H. destruct H. destruct H. rename x1 into Gl.
+  exists (g_send q p (overwrite_lis l (Some(s, Gl)) x)). 
+  split.
+  - pinversion H1; try easy. subst.
+    pfold. constructor. destruct H3.
+    clear H1 H2 H3 H4. revert H5 H0 H. clear q p pt. revert l x G' s Gl.
+    induction x0; intros; try easy.
+    - destruct l; try easy.
+    - destruct x; try easy. inversion H5. subst. clear H5.
+    - destruct l; try easy.
+      - simpl in H0. subst. destruct H4; try easy.
+      destruct H0 as (s1,(g1,(g2,(Ha,(Hb,Hc))))).
+      inversion Hb. subst.
+        constructor; try easy. right. exists s1. exists Gl. exists g2. split. easy. split. easy. left. easy.
+      - specialize(IHx0 l x G' s Gl H7 H0 H). constructor; try easy.
+    apply gttT_mon.
+    split.
+    destruct H3. intros. destruct n. exists 0. constructor.
+    specialize(H2 (S n)). specialize(H3 n). destruct H3. destruct H2.
+    exists (Nat.max x1 x2). constructor. inversion H2. subst. clear H2 H1 H0 H4 H.
+    revert H8 H3. revert n x s Gl x1 x2. clear x0 q p G' pt.
+    induction l; intros; try easy.
+    - destruct x; try easy. constructor; try easy. right. exists s. exists Gl.
+      split. easy. specialize(guardG_more n x1 (Nat.max x1 x2) Gl); intros. apply H; try easy.
+      apply max_l.
+    - inversion H8. subst. clear H8. constructor; try easy. right.
+      exists s. exists Gl. split. easy.
+      specialize(guardG_more n x1 (Nat.max x1 x2) Gl); intros. apply H; try easy. apply max_l.
+    - apply Forall_forall; intros.
+      specialize(Forall_forall (fun u : option (sort * global) =>
+        u = None \/ (exists (s : sort) (g : global), u = Some (s, g) /\ guardG n x2 g)) x); intros.
+      destruct H0. specialize(H0 H2). clear H4 H2. specialize(H0 x0 H). 
+      destruct H0. left. easy. destruct H0 as (s1,(g,(Ha,Hb))). subst. right.
+      exists s1. exists g. split. easy.
+      specialize(guardG_more n x2 (Nat.max x1 x2) g); intros. apply H0; try easy. apply max_r.
+    - destruct x; try easy.
+      specialize(IHl n nil s Gl x1 x2 H8 H3). constructor; try easy.
+      left. easy.
+    - inversion H8. subst. clear H8. specialize(IHl n x s Gl x1 x2 H2 H3). constructor; try easy.
+      destruct H1. left. easy.
+      destruct H as (s1,(g1,(Ha,Hb))). subst. right. exists s1. exists g1. split. easy.
+      specialize(guardG_more n x2 (Nat.max x1 x2) g1); intros. apply H; try easy.
+      apply max_r.
+  - case_eq (eqb pt p); intros.
+      assert (pt = p). apply eqb_eq; try easy. subst. constructor.
+    - case_eq (eqb pt q); intros.
+      assert (pt = q). apply eqb_eq; try easy. subst. constructor.
+    - assert (pt <> p). apply eqb_neq; try easy. 
+      assert (pt <> q). apply eqb_neq; try easy.
+      apply pa_sendr with (n := l) (s := s) (g := Gl); try easy.
+      apply overwriteExtract; try easy.
+Qed.
+
+Lemma part_after_step_helper3 : forall n x1 ys2 ys ys0 ys1 xs p q l s g ctxG,
+      onth n x1 = Some (s, g) -> 
+      Forall2
+        (fun (u : option (sort * global)) (v : option (sort * gtt)) =>
+         u = None /\ v = None \/
+         (exists (s : sort) (g : global) (g' : gtt),
+            u = Some (s, g) /\ v = Some (s, g') /\ upaco2 gttT bot2 g g')) x1 ys2 -> 
+      Forall2
+        (fun u v : option (sort * gtt) =>
+         u = None /\ v = None \/
+         (exists (s : sort) (g g' : gtt),
+            u = Some (s, g) /\ v = Some (s, g') /\ upaco5 gttstep bot5 g g' q p l)) ys ys2 -> 
+      Forall2
+        (fun (u : option (sort * gtt)) (v : option ltt) =>
+         u = None /\ v = None \/
+         (exists (s : sort) (g : gtt) (t : ltt),
+            u = Some (s, g) /\ v = Some t /\ upaco3 projection bot3 g q t)) ys ys0 ->
+      Forall2
+        (fun (u : option (sort * gtt)) (v : option ltt) =>
+         u = None /\ v = None \/
+         (exists (s : sort) (g : gtt) (t : ltt),
+            u = Some (s, g) /\ v = Some t /\ upaco3 projection bot3 g p t)) ys ys1 -> 
+      Forall2
+        (fun (u : option (sort * gtth)) (v : option (sort * gtt)) =>
+         u = None /\ v = None \/
+         (exists (s : sort) (g : gtth) (g' : gtt),
+            u = Some (s, g) /\ v = Some (s, g') /\ typ_gtth ctxG g g')) xs ys -> 
+      exists g' g'' t t' Gl,
+      onth n ys2 = Some (s, g') /\ gttTC g g' /\
+      onth n ys = Some (s, g'') /\ gttstepC g'' g' q p l /\
+      onth n ys0 = Some t /\ projectionC g'' q t /\
+      onth n ys1 = Some t' /\ projectionC g'' p t' /\
+      onth n xs = Some (s, Gl) /\ typ_gtth ctxG Gl g''.
+Proof.
+  induction n; intros.
+  - destruct x1; try easy. destruct ys2; try easy. destruct ys; try easy.
+    destruct ys0; try easy. destruct ys1; try easy. destruct xs; try easy.
+    inversion H0. inversion H1. inversion H2. inversion H3. inversion H4. subst. 
+    clear H0 H1 H2 H3 H4.
+    simpl in H. subst. clear H34 H28 H22 H16 H10.
+    destruct H8; try easy. destruct H. destruct H. destruct H. destruct H. destruct H0. 
+    inversion H. subst. clear H.
+    destruct H14; try easy. destruct H. destruct H. destruct H. destruct H. destruct H0. 
+    inversion H0. subst. clear H0.
+    destruct H32; try easy. destruct H. destruct H. destruct H. destruct H. destruct H0. 
+    inversion H0. subst. clear H0.
+    destruct H26; try easy. destruct H. destruct H. destruct H. destruct H. destruct H0. 
+    inversion H. subst. clear H.
+    destruct H20; try easy. destruct H. destruct H. destruct H. destruct H. destruct H0. 
+    inversion H. subst. clear H.
+    destruct H1; try easy. destruct H2; try easy. destruct H4; try easy. destruct H5; try easy.
+    simpl. exists x5. exists x6. exists x8. exists x7. exists x2. 
+    easy.
+  - destruct x1; try easy. destruct ys2; try easy. destruct ys; try easy.
+    destruct ys0; try easy. destruct ys1; try easy. destruct xs; try easy.
+    inversion H0. inversion H1. inversion H2. inversion H3. inversion H4. subst. 
+    clear H0 H1 H2 H3 H4.
+    specialize(IHn x1 ys2 ys ys0 ys1 xs p q l s g ctxG). apply IHn; try easy.
+Qed.
+
+Lemma wfgC_after_step_helper : forall n0 s G' lsg lis1, 
+      Some (s, G') = onth n0 lsg -> 
+      Forall2
+       (fun (u : option (sort * global)) (v : option (sort * gtt)) =>
+        u = None /\ v = None \/
+        (exists (s : sort) (g : global) (g' : gtt),
+           u = Some (s, g) /\ v = Some (s, g') /\ upaco2 gttT bot2 g g')) lis1 lsg -> 
+      Forall
+       (fun u : option (sort * global) =>
+        u = None \/ (exists (s : sort) (g : global), u = Some (s, g) /\ wfG g)) lis1 -> 
+      Forall
+      (fun u : option (sort * gtt) =>
+       u = None \/ (exists (s : sort) (g : gtt), u = Some (s, g) /\ balancedG g)) lsg -> 
+      Forall
+       (fun u : option (sort * global) =>
+        u = None \/
+        (exists (s : sort) (g : global),
+           u = Some (s, g) /\ (forall n : fin, exists m : fin, guardG n m g))) lis1 -> 
+      exists G1, onth n0 lis1 = Some(s, G1) /\ gttTC G1 G' /\ wfG G1 /\ balancedG G' /\ (forall n, exists m, guardG n m G1).
+Proof.
+  induction n0; intros.
+  - destruct lsg; try easy. destruct lis1; try easy.
+    inversion H0. subst. clear H0. inversion H1. subst. clear H1. inversion H2. subst. clear H2.
+    inversion H3. subst. clear H3. 
+    simpl in H. subst.
+    destruct H7; try easy. destruct H as (s0,(g1,(g2,(Ha,(Hb,Hc))))). inversion Hb. subst.
+    destruct H5; try easy. destruct H as (s1,(g3,(Hd,He))). inversion Hd. subst.
+    destruct H4; try easy. destruct H as (s2,(g4,(Hf,Hg))). inversion Hf. subst.
+    destruct H2; try easy. destruct H as (s3,(g5,(Hh,Hi))). inversion Hh. subst.
+    simpl. exists g5. pclearbot. easy.
+  - destruct lsg; try easy. destruct lis1; try easy.
+    inversion H0. subst. clear H0. inversion H1. subst. clear H1. inversion H2. subst. clear H2.
+    inversion H3. subst. clear H3. 
+    specialize(IHn0 s G' lsg lis1). apply IHn0; try easy.
+Qed.
+
+Lemma wfgC_after_step_helper2 : forall lis ys ys0 n p q,
+    SList lis -> 
+    Forall2
+       (fun (u : option (sort * global)) (v : option (sort * gtt)) =>
+        u = None /\ v = None \/
+        (exists (s : sort) (g : global) (g' : gtt),
+           u = Some (s, g) /\ v = Some (s, g') /\ upaco2 gttT bot2 g g')) lis ys -> 
+    Forall2
+        (fun u v : option (sort * gtt) =>
+         u = None /\ v = None \/
+         (exists (s : sort) (g g' : gtt),
+            u = Some (s, g) /\ v = Some (s, g') /\ upaco5 gttstep bot5 g g' p q n))
+        ys ys0 ->
+    SList ys0.
+Proof.
+  induction lis; intros; try easy.
+  specialize(SList_f a lis H); intros. destruct ys; try easy. destruct ys0; try easy.
+  specialize(IHlis ys ys0 n p q). inversion H0. subst. clear H0. inversion H1. subst. clear H1.
+  destruct H2. apply SList_b. apply IHlis; try easy.
+  destruct H0. destruct H1. subst. destruct H6; try easy.
+  destruct H0 as (s0,(g0,(g1,(Ha,(Hb,Hc))))). subst. destruct ys; try easy.
+  destruct H5; try easy. destruct H0 as (s2,(g2,(g3,(Hta,(Htb,Htc))))). inversion Hta. subst.
+  destruct ys0; try easy.
+Qed.
+
+Lemma wfgC_after_step_helper3 : forall ys0 xs,
+      SList ys0 -> 
+      Forall2
+       (fun (u : option (sort * global)) (v : option (sort * gtt)) =>
+        u = None /\ v = None \/
+        (exists (s : sort) (g : global) (g' : gtt),
+           u = Some (s, g) /\ v = Some (s, g') /\ gttTC g g')) xs ys0 -> 
+      SList xs.
+Proof.
+  induction ys0; intros; try easy.
+  specialize(SList_f a ys0 H); intros. 
+  destruct xs; try easy.
+  specialize(IHys0 xs). inversion H0. subst. clear H0.
+  destruct H1. apply SList_b. apply IHys0; try easy.
+  destruct H0. destruct H1. subst.
+  destruct H5; try easy. destruct H0 as (s,(g,(g',(Ha,(Hb,Hc))))). inversion Hb. subst.
+  destruct xs; try easy.
+Qed.
