slem/subtype.v
@@ -1,0 +1,262 @@
+From mathcomp Require Import ssreflect.seq all_ssreflect.
+From Paco Require Import paco pacotac.
+From SST Require Export src.expressions src.header src.local src.mono.
+Require Import List String Coq.Arith.PeanoNat Morphisms Relations.
+Import ListNotations. 
+
+Lemma refl_recv: forall (l1:  list (option(sort*ltt))) (R1: sort -> sort -> Prop) (R2: ltt -> ltt -> Prop),
+   Reflexive R1 -> Reflexive R2 ->
+   wfrec R1 R2 l1 l1.
+Proof. intro l1.
+       induction l1; intros.
+       - simpl. easy.
+       - simpl. destruct a. destruct p.
+         split. reflexivity.
+         split. reflexivity.
+         apply IHl1.
+         easy. easy.
+         apply IHl1.
+         easy. easy.
+Qed.
+
+Lemma refl_send: forall (l1:  list (option(sort*ltt))) (R1: sort -> sort -> Prop) (R2: ltt -> ltt -> Prop),
+   Reflexive R1 -> Reflexive R2 ->
+   wfsend R1 R2 l1 l1.
+Proof. intro l1.
+       induction l1; intros.
+       - simpl. easy.
+       - simpl. destruct a. destruct p.
+         split. reflexivity.
+         split. reflexivity.
+         apply IHl1.
+         easy. easy.
+         apply IHl1.
+         easy. easy.
+Qed.
+
+Lemma stRefl: forall l, subtypeC l l.
+Proof. pcofix CIH.
+       intros.
+       pfold.
+       case_eq l; intros.
+       constructor.
+       constructor.
+       apply refl_recv.
+       constructor.
+
+       repeat intro.
+       unfold upaco2.
+       right. apply CIH.
+
+       constructor.
+       apply refl_send.
+       constructor.
+       repeat intro.
+       right. apply CIH.
+Qed.
+
+Lemma subtype_end : forall H, subtypeC ltt_end H -> H = ltt_end.
+Proof.
+  intros. punfold H0. inversion H0. easy. 
+  apply subtype_monotone.
+Qed.
+
+Lemma subtype_recv_inv_helper : forall pt s s0 l l0 xs ys,
+    subtypeC (ltt_recv pt (Some (s, l) :: xs)) (ltt_recv pt (Some (s0, l0) :: ys)) -> 
+    subtypeC l l0.
+Proof.
+  intros. 
+  pinversion H. subst.
+  simpl in H1.
+  destruct H1. destruct H1.
+  pclearbot.
+  unfold subtypeC. easy.
+  apply subtype_monotone.
+Qed.
+
+Lemma subtype_recv_inv : forall pt xs ys, subtypeC (ltt_recv pt xs) (ltt_recv pt ys) -> Forall2R (fun u v => (u = None) \/ (exists s s' t t', u = Some(s,t) /\ v = Some (s',t') /\ subsort s s' /\ subtypeC t' t)) ys xs.
+Proof.
+  intros pt xs ys. revert pt xs.
+  induction ys; intros. constructor.
+  - destruct xs; try easy.
+    pinversion H. subst. 
+    simpl in H1. destruct a. destruct p. easy. easy.
+    apply subtype_monotone.
+  constructor.
+  - destruct o. destruct a. destruct p0. destruct p. right.
+    exists s. exists s0. exists l. exists l0. split; try easy. split; try easy.
+    split. 
+    pinversion H. subst. destruct H1. easy.
+    apply subtype_monotone.
+    specialize(subtype_recv_inv_helper pt s0 s l0 l xs ys H); intros. easy.
+    left. easy.
+    pinversion H. subst. 
+    simpl in H1. destruct a; try easy.
+    destruct p. easy.
+    left. easy.
+    apply subtype_monotone.
+  - apply IHys with (pt := pt).
+    pinversion H. subst. 
+    pfold. constructor.
+    simpl in H1. 
+    destruct o. destruct p. destruct a. destruct p. destruct H1. destruct H1. easy. easy.
+    destruct a. destruct p. easy. easy.
+  - apply subtype_monotone.
+Qed.
+
+Lemma subtype_recv : forall H pt xs, subtypeC (ltt_recv pt xs) H -> (exists ys, 
+                    H = ltt_recv pt ys).
+Proof.
+  induction xs; intros; try easy.
+  - pinversion H0. subst. exists ys. easy.
+    apply subtype_monotone.
+  - destruct H.
+    pinversion H0. apply subtype_monotone.
+    pinversion H0. subst. exists l. easy. apply subtype_monotone.
+    pinversion H0. apply subtype_monotone.
+Qed.
+
+Lemma subtype_send_inv_helper : forall pt s s0 l l0 xs ys,
+    subtypeC (ltt_send pt (Some (s, l) :: xs)) (ltt_send pt (Some (s0, l0) :: ys)) -> 
+    subtypeC l l0.
+Proof.
+  intros. 
+  pinversion H. subst.
+  simpl in H1.
+  destruct H1. destruct H1.
+  pclearbot.
+  unfold subtypeC. easy.
+  apply subtype_monotone.
+Qed.
+
+Lemma subtype_send_inv : forall pt xs ys, subtypeC (ltt_send pt xs) (ltt_send pt ys) -> Forall2R (fun u v => (u = None) \/ (exists s s' t t', u = Some(s,t) /\ v = Some (s',t') /\ subsort s s' /\ subtypeC t t')) xs ys.
+Proof.
+  induction xs; intros.
+  - constructor.
+  - destruct ys; try easy.
+    pinversion H. subst. simpl in H1. destruct a. destruct p. easy. easy.
+    apply subtype_monotone.
+  constructor.
+  - destruct a. right. destruct p. destruct o. destruct p.
+    exists s. exists s0. exists l. exists l0. split; try easy. split; try easy.
+    split.
+    pinversion H. subst. simpl in H1. destruct H1. easy.
+    apply subtype_monotone.
+    specialize(subtype_send_inv_helper pt s s0 l l0 xs ys H); intros. easy.
+    pinversion H. subst. simpl in H1. easy.
+  - apply subtype_monotone.
+    left. easy.
+  - apply IHxs.
+    pinversion H. subst. 
+    pfold. constructor.
+    simpl in H1. 
+    destruct o. destruct p. destruct a. destruct p. destruct H1. destruct H1. easy. easy.
+    destruct a. destruct p. easy. easy.
+  - apply subtype_monotone.
+Qed.
+
+Lemma subtype_send : forall H pt xs, subtypeC (ltt_send pt xs) H -> (exists ys, 
+                    H = ltt_send pt ys).
+Proof.
+  induction xs; intros; try easy.
+  - pinversion H0. subst. exists ys. easy.
+    apply subtype_monotone.
+  - destruct H.
+    pinversion H0. apply subtype_monotone.
+    pinversion H0. apply subtype_monotone.
+    pinversion H0. subst. exists l. easy. apply subtype_monotone.
+Qed.
+
+Lemma stTrans_helper_recv : forall x x0 l r,
+      (forall l1 l2 l3 : ltt, subtypeC l1 l2 -> subtypeC l2 l3 -> r l1 l3) ->
+      Forall2R
+      (fun u v : option (sort * ltt) =>
+       u = None \/
+       (exists (s s' : sort) (t t' : ltt),
+          u = Some (s, t) /\ v = Some (s', t') /\ subsort s s' /\ subtypeC t' t)) x0 x ->
+      Forall2R
+       (fun u v : option (sort * ltt) =>
+        u = None \/
+        (exists (s s' : sort) (t t' : ltt),
+           u = Some (s, t) /\ v = Some (s', t') /\ subsort s s' /\ subtypeC t' t)) x l ->
+      wfrec subsort (upaco2 subtype r) x0 l.
+Proof.
+  induction x; intros; try easy.
+  destruct x0; try easy. 
+  destruct l; try easy. destruct x0; try easy.
+  inversion H0; subst. clear H0. inversion H1. subst. clear H1.
+  simpl.
+  destruct H5. 
+  - subst. destruct o. destruct p. apply IHx; try easy. apply IHx; try easy.
+  - destruct H0. destruct H0. destruct H0. destruct H0. destruct H0. destruct H1. destruct H2.
+    subst.
+    destruct H4; try easy. destruct H0. destruct H0. destruct H0. destruct H0. destruct H0. destruct H1. destruct H4.
+    inversion H0.
+    subst.
+    split. apply sstrans with (s2 := x5); try easy.
+    split. unfold upaco2. right. apply H with (l2 := x7); try easy. 
+    apply IHx; try easy.
+Qed. 
+
+Lemma stTrans_helper_send : forall x x0 l r,
+      (forall l1 l2 l3 : ltt, subtypeC l1 l2 -> subtypeC l2 l3 -> r l1 l3) ->
+      Forall2R
+      (fun u v : option (sort * ltt) =>
+       u = None \/
+       (exists (s s' : sort) (t t' : ltt),
+          u = Some (s, t) /\ v = Some (s', t') /\ subsort s s' /\ subtypeC t t')) x x0 -> 
+      Forall2R
+       (fun u v : option (sort * ltt) =>
+        u = None \/
+        (exists (s s' : sort) (t t' : ltt),
+           u = Some (s, t) /\ v = Some (s', t') /\ subsort s s' /\ subtypeC t t')) l x ->
+      wfsend subsort (upaco2 subtype r) l x0.
+Proof.
+  induction x; intros; try easy.
+  destruct l; try easy.
+  destruct l; try easy. destruct x0; try easy.
+  inversion H0; subst. clear H0. inversion H1. subst. clear H1.
+  simpl.
+  destruct H5. 
+  - subst. destruct o. destruct p. destruct H4. easy. destruct H0. destruct H0. 
+    destruct H0. destruct H0. destruct H0. destruct H1. easy.
+    destruct o0. destruct p. apply IHx; try easy. apply IHx; try easy.
+  - destruct H0. destruct H0. destruct H0. destruct H0. destruct H0. destruct H1. destruct H2.
+    subst.
+    destruct H4. subst. apply IHx; try easy. 
+    destruct H0. destruct H0. destruct H0. destruct H0. destruct H0. destruct H1. destruct H4.
+    subst.
+    inversion H1. subst.
+    split. apply sstrans with (s2 := x6); try easy.
+    split. unfold upaco2. right. apply H with (l2 := x8); try easy.
+    apply IHx; try easy.
+Qed. 
+
+Lemma stTrans: forall l1 l2 l3, subtypeC l1 l2 -> subtypeC l2 l3 -> subtypeC l1 l3.
+  Proof.
+    pcofix CIH. intros.
+    pfold. case_eq l1; intros.
+    - subst. 
+      specialize(subtype_end l2 H0); intros. subst.
+      specialize(subtype_end l3 H1); intros. subst. apply sub_end.
+    - subst.
+      specialize(subtype_recv l2 s l H0); intros. destruct H. subst.
+      specialize(subtype_recv l3 s x H1); intros. destruct H. subst.
+      
+      specialize(subtype_recv_inv s x x0 H1); intros.
+      specialize(subtype_recv_inv s l x H0); intros.
+      
+      constructor.
+      
+      apply stTrans_helper_recv with (x := x); try easy.
+      
+    - subst.
+      specialize(subtype_send l2 s l H0); intros. destruct H. subst.
+      specialize(subtype_send l3 s x H1); intros. destruct H. subst.
+      
+      specialize(subtype_send_inv s x x0 H1); intros.
+      specialize(subtype_send_inv s l x H0); intros.
+      
+      constructor.
+      apply stTrans_helper_send with (x := x); try easy.
+Qed.
