src/global.v
@@ -1,0 +1,104 @@
+From mathcomp Require Import ssreflect.seq all_ssreflect.
+From Paco Require Import paco pacotac.
+From SST Require Export src.expressions src.header.
+Require Import List String Coq.Arith.PeanoNat Relations. 
+Import ListNotations. 
+
+Section gtt.
+
+(* global session trees *)
+CoInductive gtt: Type :=
+  | gtt_end    : gtt
+  | gtt_send   : part -> part -> list (option (sort*gtt)) -> gtt.
+
+Definition gtt_id (s: gtt): gtt :=
+  match s with
+    | gtt_end        => gtt_end
+    | gtt_send p q l => gtt_send p q l
+  end.
+
+Lemma gtt_eq: forall s, s = gtt_id s.
+Proof. intro s; destruct s; easy. Defined.
+
+Inductive global  : Type :=
+  | g_var : fin -> global 
+  | g_end : global 
+  | g_send : part -> part -> list (option (sort * global)) -> global 
+  | g_rec : global -> global.
+  
+Section global_ind_ref.
+  Variable P : global -> Prop.
+  Hypothesis P_var : forall n, P (g_var n).
+  Hypothesis P_end : P (g_end).
+  Hypothesis P_send : forall p q lis, List.Forall (fun u => u = None \/ (exists s g, u = Some (s, g) /\ P g)) lis -> P (g_send p q lis).
+  Hypothesis P_rec : forall g, P g -> P (g_rec g).
+  
+  Fixpoint global_ind_ref p : P p.
+  Proof.
+    destruct p.
+    - apply P_var.
+    - apply P_end.
+    - apply P_send.
+      induction l; try easy.
+      constructor; try easy.
+      destruct a. right. destruct p. exists s1. exists g. split; try easy.
+      left. easy.
+    - apply P_rec. easy.
+  Qed.
+End global_ind_ref.
+
+Fixpoint incr_freeG (fv m : fin) (G : global) := 
+  match G with 
+    | g_var n        => g_var (if fv <= n then (n + m) else n)
+    | g_end          => g_end 
+    | g_send p q lis => g_send p q (map (fun u => 
+          match u with 
+            | Some (s, g) => Some (s, incr_freeG fv m g)
+            | None        => None
+          end) lis)
+    | g_rec g        => g_rec (incr_freeG (S fv) m g)
+  end.
+
+Inductive subst_global : fin -> fin -> global -> global -> global -> Prop := 
+  | subg_var_is   : forall G t m,                            subst_global t m G (g_var t) (incr_freeG 0 m G)
+  | subg_var_notz : forall G t m, t <> 0 ->                  subst_global t m G (g_var 0) (g_var 0)
+  | subg_var_not1 : forall G t t' m, t <> S t' -> t <= t' -> subst_global t m G (g_var (S t')) (g_var (t'))
+  | subg_var_not2 : forall G t t' m, t <> S t' -> t' < t  -> subst_global t m G (g_var (S t')) (g_var (S t'))
+  | subg_end      : forall G t m,                            subst_global t m G g_end g_end
+  | subg_send     : forall G t m p q xs ys, List.Forall2 (fun u v => 
+                           (u = None /\ v = None) \/
+                           (exists s g g', u = Some(s, g) /\ v = Some(s, g') /\ subst_global t m G g g')
+                                                  ) xs ys -> subst_global t m G (g_send p q xs) (g_send p q ys)
+  | subg_rec      : forall G t m P Q, subst_global (S t) (S m) G P Q -> subst_global t m G (g_rec P) (g_rec Q). 
+
+Inductive betaG : relation global := 
+  | lttS : forall G G', subst_global 0 0 (g_rec G) G G' -> betaG (g_rec G) G'.
+
+Inductive gttT (R : global -> gtt -> Prop) : global -> gtt -> Prop := 
+  | gttT_end  : gttT R g_end gtt_end
+  | gttT_send : forall p q xs ys, List.Forall2 (fun u v => (u = None /\ v = None) \/ (exists s g g', u = Some(s, g) /\ v = Some(s, g') /\ R g g')) xs ys -> gttT R (g_send p q xs) (gtt_send p q ys)
+  | gttT_rec  : forall G Q G', subst_global 0 0 (g_rec G) G Q -> R Q G' -> gttT R (g_rec G) G'.
+
+Definition gttTC G G' := paco2 gttT bot2 G G'.
+
+Inductive wfG : global -> Prop := 
+  | wfg_var : forall n, wfG (g_var n)
+  | wfg_end : wfG g_end
+  | wfg_send : forall p q lis, SList lis -> p <> q -> List.Forall (fun u => u = None \/ (exists s g, u = Some(s, g) /\ wfG g)) lis -> wfG (g_send p q lis)
+  | wfg_rec : forall g, wfG g -> wfG (g_rec g).
+
+Inductive guardG : fin -> fin -> global -> Prop :=  
+  | gg_nil : forall m G, guardG 0 m G
+  | gg_end : forall n m, guardG n m g_end
+  | gg_send : forall n m p q lis, List.Forall (fun u => u = None \/ (exists s g, u = Some(s, g) /\ guardG n m g)) lis -> guardG (S n) m (g_send p q lis)
+  | gg_rec : forall n m g Q, subst_global 0 0 (g_rec g) g Q -> guardG n m Q -> guardG n (S m) (g_rec g).
+
+End gtt.
+
+
+
+
+
+
+
+
