src/local.v
@@ -1,0 +1,145 @@
+From mathcomp Require Import ssreflect.seq all_ssreflect.
+From Paco Require Import paco pacotac.
+From SST Require Export src.expressions src.header.
+Require Import List String Coq.Arith.PeanoNat Morphisms Relations.
+Import ListNotations. 
+
+Section ltt.
+
+CoInductive ltt: Type :=
+  | ltt_end : ltt
+  | ltt_recv: part -> list (option(sort*ltt)) -> ltt
+  | ltt_send: part -> list (option(sort*ltt)) -> ltt.
+
+Definition ltt_id (s: ltt): ltt :=
+  match s with
+    | ltt_end      => ltt_end
+    | ltt_recv p l => ltt_recv p l 
+    | ltt_send p l => ltt_send p l
+  end.
+  
+Lemma ltt_eq: forall s, s = ltt_id s.
+Proof. intro s; destruct s; easy. Defined.
+
+Inductive local  : Type :=
+  | l_var : fin -> local 
+  | l_end : local 
+  | l_send : part -> list (option (sort * local)) -> local 
+  | l_recv : part -> list (option (sort * local)) -> local 
+  | l_rec : local -> local .
+  
+Section local_ind_ref.
+  Variable P : local -> Prop.
+  Hypothesis P_var : forall n, P (l_var n).
+  Hypothesis P_end : P (l_end).
+  Hypothesis P_send : forall p lis, List.Forall (fun u => u = None \/ (exists s g, u = Some (s, g) /\ P g)) lis -> P (l_send p lis).
+  Hypothesis P_recv : forall p lis, List.Forall (fun u => u = None \/ (exists s g, u = Some (s, g) /\ P g)) lis -> P (l_recv p lis).
+  Hypothesis P_rec : forall g, P g -> P (l_rec g).
+
+  Fixpoint local_ind_ref p : P p.
+  Proof.
+    destruct p.
+    - apply P_var.
+    - apply P_end.
+    - apply P_send.
+      induction l; try easy.
+      constructor; try easy.
+      destruct a. right. destruct p. exists s0. exists l0. split; try easy.
+      left. easy.
+    - apply P_recv.
+      induction l; try easy.
+      constructor; try easy.
+      destruct a. right. destruct p. exists s0. exists l0. split; try easy.
+      left. easy.
+    - apply P_rec; easy.
+  Qed.
+End local_ind_ref.
+
+Fixpoint incr_freeL (fv m : fin) (T : local) := 
+  match T with 
+    | l_var n        => l_var (if fv <= n then (n + m) else n)
+    | l_end          => l_end 
+    | l_send p lis => l_send p (List.map (fun u => 
+          match u with 
+            | Some (s, g) => Some (s, incr_freeL fv m g)
+            | None        => None
+          end) lis)
+    | l_recv p lis => l_recv p (List.map (fun u => 
+          match u with 
+            | Some (s, g) => Some (s, incr_freeL fv m g)
+            | None        => None
+          end) lis)
+    | l_rec g        => l_rec (incr_freeL (S fv) m g)
+  end.
+
+Inductive subst_local : fin -> fin -> local -> local -> local -> Prop := 
+  | subl_var_is   : forall G t m,                            subst_local t m G (l_var t) (incr_freeL 0 m G)
+  | subl_var_notz : forall G t m, t <> 0 ->                  subst_local t m G (l_var 0) (l_var 0)
+  | subl_var_not1 : forall G t t' m, t <> S t' -> t <= t' -> subst_local t m G (l_var (S t')) (l_var (t'))
+  | subl_var_not2 : forall G t t' m, t <> S t' -> t' < t  -> subst_local t m G (l_var (S t')) (l_var (S t'))
+  | subl_end      : forall G t m,                            subst_local t m G l_end l_end
+  | subl_send     : forall G t m p xs ys, List.Forall2 (fun u v => 
+                           (u = None /\ v = None) \/
+                           (exists s g g', u = Some(s, g) /\ v = Some(s, g') /\ subst_local t m G g g')
+                                                  ) xs ys -> subst_local t m G (l_send p xs) (l_send p ys)
+  | subl_recv     : forall G t m p xs ys, List.Forall2 (fun u v => 
+                           (u = None /\ v = None) \/
+                           (exists s g g', u = Some(s, g) /\ v = Some(s, g') /\ subst_local t m G g g')
+                                                  ) xs ys -> subst_local t m G (l_recv p xs) (l_recv p ys)
+  | subl_rec      : forall G t m P Q, subst_local (S t) (S m) G P Q -> subst_local t m G (l_rec P) (l_rec Q). 
+
+Inductive betaL : relation local := 
+  | lttS : forall G G', subst_local 0 0 (l_rec G) G G' -> betaL (l_rec G) G'.
+
+Inductive lttT (R : local -> ltt -> Prop) : local -> ltt -> Prop := 
+  | lttT_end  : lttT R l_end ltt_end
+  | lttT_send : forall p xs ys, List.Forall2 (fun u v => (u = None /\ v = None) \/ (exists s g g', u = Some(s, g) /\ v = Some(s, g') /\ R g g')) xs ys -> lttT R (l_send p xs) (ltt_send p ys)
+  | lttT_recv : forall p xs ys, List.Forall2 (fun u v => (u = None /\ v = None) \/ (exists s g g', u = Some(s, g) /\ v = Some(s, g') /\ R g g')) xs ys -> lttT R (l_recv p xs) (ltt_recv p ys)
+  | lttT_rec  : forall G Q G', subst_local 0 0 (l_rec G) G Q -> lttT R Q G' -> lttT R (l_rec G) G'.
+
+Definition lttTC G G' := paco2 lttT bot2 G G'.
+
+Inductive wfL : local -> Prop :=
+  | wfl_var : forall n, wfL (l_var n)
+  | wfl_end : wfL l_end
+  | wfl_send : forall p lis, SList lis -> List.Forall (fun u => u = None \/ (exists s g, u = Some(s, g) /\ wfL g)) lis -> wfL (l_send p lis)
+  | wfl_recv : forall p lis, SList lis -> List.Forall (fun u => u = None \/ (exists s g, u = Some(s, g) /\ wfL g)) lis -> wfL (l_recv p lis)
+  | wfl_rec  : forall g, wfL g -> wfL (l_rec g).
+
+Inductive guardL : fin -> fin -> local -> Prop := 
+  | gl_nil  : forall m T, guardL 0 m T
+  | gl_end  : forall n m, guardL n m l_end
+  | gl_send : forall n m p lis, List.Forall (fun u => u = None \/ (exists s g, u = Some(s, g) /\ guardL n m g)) lis -> guardL (S n) m (l_send p lis)
+  | gl_recv : forall n m p lis, List.Forall (fun u => u = None \/ (exists s g, u = Some(s, g) /\ guardL n m g)) lis -> guardL (S n) m (l_recv p lis)
+  | gl_rec  : forall n m g Q, subst_local 0 0 (l_rec g) g Q -> guardL n m Q -> guardL n (S m) (l_rec g).
+
+Fixpoint wfrec (R1: sort -> sort -> Prop) (R2: ltt -> ltt -> Prop) (l1 l2: list (option(sort*ltt))): Prop :=
+  match (l1,l2) with
+    | (Datatypes.None::xs, Datatypes.None::ys)               => wfrec R1 R2 xs ys
+    | (Datatypes.Some (s',t')::xs, Datatypes.Some (s,t)::ys) => R1 s' s /\ R2 t t' /\ wfrec R1 R2 xs ys
+    | (Datatypes.None::xs, Datatypes.Some(s,t)::ys)          => wfrec R1 R2 xs ys
+    | (nil, _)                                               => True
+    | _                                                      => False
+  end.
+
+Fixpoint wfsend (R1: sort -> sort -> Prop) (R2: ltt -> ltt -> Prop) (l1 l2: list (option(sort*ltt))): Prop :=
+  match (l1,l2) with
+    | (Datatypes.None::xs, Datatypes.None::ys)               => wfsend R1 R2 xs ys
+    | (Datatypes.Some (s,t)::xs, Datatypes.Some (s',t')::ys) => R1 s s' /\ R2 t t' /\ wfsend R1 R2 xs ys
+    | (Datatypes.None::xs, Datatypes.Some(s',t')::ys)        => wfsend R1 R2 xs ys
+    | (nil, _)                                               => True
+    | _                                                      => False
+  end.
+
+Inductive subtype (R: ltt -> ltt -> Prop): ltt -> ltt -> Prop :=
+  | sub_end: subtype R ltt_end ltt_end
+  | sub_in : forall p xs ys,
+                    wfrec subsort R ys xs ->
+                    subtype R (ltt_recv p xs) (ltt_recv p ys)
+  | sub_out : forall p xs ys,
+                     wfsend subsort R xs ys ->
+                     subtype R (ltt_send p xs) (ltt_send p ys).
+
+Definition subtypeC l1 l2 := paco2 subtype bot2 l1 l2.
+
+End ltt.
