src/merge.v
@@ -1,0 +1,11 @@
+From SST Require Export type.global type.local type.isomorphism.
+Require Import List String Datatypes ZArith Relations PeanoNat.
+Open Scope list_scope.
+From Paco Require Import paco pacotac.
+Require Import Setoid Morphisms Coq.Program.Basics.
+Require Import Coq.Init.Datatypes.
+
+Inductive isMerge : ltt -> list (option ltt) -> Prop :=
+  | matm : forall t, isMerge t (Some t :: nil)
+  | mconsn : forall t xs, isMerge t xs -> isMerge t (None :: xs) 
+  | mconss : forall t xs, isMerge t xs -> isMerge t (Some t :: xs). 
