src/mono.v
@@ -1,0 +1,149 @@
+From mathcomp Require Import ssreflect.seq all_ssreflect.
+Require Import List String Coq.Arith.PeanoNat Relations.
+Import ListNotations. 
+From SST Require Import src.header src.local src.global. 
+
+Definition Forall_mono {X} {R T : X -> Prop} (HRT : forall x, R x -> T x) :
+      forall l, Forall R l -> Forall T l.
+Proof.
+  induction l; intros; try easy.
+  inversion H. subst. specialize(IHl H3). constructor; try easy.
+  apply HRT; try easy.
+Qed.
+
+Definition Forall2_mono {X Y} {R T : X -> Y -> Prop} (HRT : forall x y, R x y -> T x y) :
+      forall l m, Forall2 R l m -> Forall2 T l m :=
+  fix loop l m h {struct h} :=
+    match h with
+    | Forall2_nil => Forall2_nil T
+    | Forall2_cons _ _ _ _ h1 h2 => Forall2_cons _ _ (HRT _ _ h1) (loop _ _ h2)
+    end.
+
+Definition Forall2R_mono {X Y} {R T : X -> Y -> Prop} (HRT : forall x y, R x y -> T x y) :
+      forall l m, Forall2R R l m -> Forall2R T l m :=
+  fix loop l m h {struct h} :=
+    match h with
+    | Forall2R_nil xs => Forall2R_nil T xs
+    | Forall2R_cons _ _ _ _ h1 h2 => Forall2R_cons _ _ _ _ _ (HRT _ _ h1) (loop _ _ h2)
+    end.
+
+Lemma subtype_monotone : monotone2 subtype.
+Proof.
+  unfold monotone2.
+  intros. induction IN; intros.
+  - constructor.
+  - constructor.
+    revert H. revert ys. 
+    induction xs. destruct ys; try easy.
+    intros. destruct ys; try easy. simpl.
+    simpl in H. destruct o; try easy. destruct p0. destruct a; try easy. destruct p0.
+    destruct H. destruct H0. split; try easy. split; try easy. apply LE; try easy. apply IHxs; try easy.
+    destruct a; try easy. destruct p0. apply IHxs; try easy. apply IHxs; try easy. 
+  - constructor.
+    revert H. revert ys.
+    induction xs. destruct ys; try easy.
+    intros. destruct ys; try easy. simpl in *.
+    destruct a; try easy. destruct p0. destruct o; try easy. destruct p0. 
+    destruct H. destruct H0. split; try easy. split. apply LE; try easy. apply IHxs; try easy.
+    destruct o; try easy. destruct p0. apply IHxs; try easy. apply IHxs; try easy.
+Qed.
+
+Lemma lttT_mon : monotone2 lttT.
+Proof.
+  unfold monotone2. intros. induction IN; intros; try easy.
+  - apply lttT_end.
+  - apply lttT_send; try easy.
+    - revert H LE. revert r r' p ys.
+      induction xs; intros; try easy.
+      destruct ys; try easy.
+      destruct ys; try easy.
+      inversion H. subst.
+      constructor.
+      - destruct H3. left. easy.
+        destruct H0. destruct H0. destruct H0. destruct H0. destruct H1. subst. right.
+        exists x. exists x0. exists x1. split; try easy. split; try easy.
+        apply LE; try easy.
+      - apply IHxs with (r := r); try easy.
+  - apply lttT_recv; try easy.
+    - revert H LE. revert r r' p ys.
+      induction xs; intros; try easy.
+      destruct ys; try easy.
+      destruct ys; try easy.
+      inversion H. subst.
+      constructor.
+      - destruct H3. left. easy.
+        destruct H0. destruct H0. destruct H0. destruct H0. destruct H1. subst. right.
+        exists x. exists x0. exists x1. split; try easy. split; try easy.
+        apply LE; try easy.
+      - apply IHxs with (r := r); try easy.
+  - apply lttT_rec with (Q := Q); try easy.
+
+Qed.
+
+Lemma gttT_mon : monotone2 gttT.
+Proof.
+  unfold monotone2. intros.
+  induction IN; intros; try easy.
+  - apply gttT_end.
+  - apply gttT_send; try easy.
+    - revert H LE. revert r r' p q ys.
+      induction xs; intros; try easy.
+      destruct ys; try easy.
+      destruct ys; try easy.
+      inversion H. subst.
+      constructor.
+      - destruct H3. left. easy.
+        destruct H0. destruct H0. destruct H0. destruct H0. destruct H1. subst. right.
+        exists x. exists x0. exists x1. split; try easy. split; try easy.
+        apply LE; try easy.
+      - apply IHxs with (r := r); try easy.
+  - apply gttT_rec with (Q := Q); try easy.
+    apply LE; try easy.
+Qed.
+
+Lemma Iso_mon : monotone2 lttIso.
+Proof.
+  unfold monotone2; intros.
+  induction IN; intros; try easy.
+  - constructor.
+  - constructor. revert H. revert xs ys.
+    induction xs; intros; try easy. destruct ys; try easy.
+    destruct a. destruct p0. destruct o; try easy. destruct p0.
+    simpl in *. split. easy. split. apply LE; try easy.
+    apply IHxs; try easy.
+  - destruct o; try easy.
+    apply IHxs; try easy.
+  - constructor. revert H. revert xs ys.
+    induction xs; intros; try easy. destruct ys; try easy.
+    destruct a. destruct p0. destruct o; try easy. destruct p0.
+    simpl in *. split. easy. split. apply LE; try easy.
+    apply IHxs; try easy.
+  - destruct o; try easy.
+    apply IHxs; try easy.
+Qed.
+
+Lemma step_mon : monotone5 gttstep.
+Proof. unfold monotone5.
+       intros.
+       induction IN; intros.
+       - apply steq with (s := s). easy. easy.
+       - constructor; try easy. 
+         revert ys H6.
+         induction xs; intros.
+         + subst. inversion H6. constructor.
+         + subst. inversion H6. constructor.
+           subst.
+           destruct H9 as [(H9a, H9b) | (s1,(g,(t,(Ht1,(Ht2,Ht3)))))].
+           subst. left. easy.
+           subst. right. exists s1. exists g. exists t.
+           split. easy. split. easy. apply LE. easy.
+           apply IHxs.
+           rewrite Forall_forall.
+           intros u Hu.
+           subst. rewrite Forall_forall in H5.
+           specialize(H5 u).
+           assert(In u (a :: xs)) by (simpl; right; easy).
+           apply H5 in H7.
+           easy.
+           easy.
+Qed.
