src/step.v
@@ -1,0 +1,24 @@
+From mathcomp Require Import ssreflect.seq all_ssreflect.
+From Paco Require Import paco pacotac.
+From SST Require Export src.expressions src.header src.global src.local src.merge src.global_tree_ctx src.projection.
+Require Import List String Coq.Arith.PeanoNat Relations Coq.Logic.Decidable.
+Import ListNotations. 
+
+Variant gttstep (R: gtt -> gtt -> part -> part -> nat -> Prop): gtt -> gtt -> part -> part -> nat -> Prop :=
+  | steq : forall p q xs s gc n,
+                  p <> q ->
+                  Datatypes.Some (s, gc) = onth n xs ->
+                  gttstep R (gtt_send p q xs) gc p q n
+  | stneq: forall p q r s xs ys n,
+                  p <> q ->
+                  r <> s ->
+                  r <> p ->
+                  r <> q ->
+                  s <> p ->
+                  s <> q ->
+                  List.Forall (fun u => u = None \/ (exists s g, u = Some(s, g) /\ isgPartsC p g /\ isgPartsC q g)) xs ->
+                  List.Forall2 (fun u v => (u = None /\ v = None) \/ (exists s g g', u = Some(s, g) /\ v = Some(s, g') /\ R g g' p q n)) xs ys ->
+                  gttstep R (gtt_send r s xs) (gtt_send r s ys) p q n.
+
+Definition gttstepC g1 g2 p q n := paco5 gttstep bot5 g1 g2 p q n. 
+
