theo/step.v
@@ -1,0 +1,309 @@
+From mathcomp Require Import ssreflect.seq all_ssreflect.
+From Paco Require Import paco pacotac.
+From SST Require Export src.expressions src.header src.global src.local src.merge src.global_tree_ctx src.projection slem.step.
+Require Import List String Coq.Arith.PeanoNat Relations Coq.Logic.Decidable.
+Import ListNotations. 
+
+Lemma part_after_step : forall G G' q p pt l LP LQ,
+        wfgC G ->
+        wfgC G' -> 
+        gttstepC G G' q p l -> 
+        projectionC G p (ltt_recv q LQ) ->
+        projectionC G q (ltt_send p LP) ->
+        isgPartsC pt G' -> 
+        isgPartsC pt G.
+Proof.
+  intros.
+  specialize(_a_29_11 G q p LP H H3); intros.
+  destruct H5 as (Gl,(ctxG,(Ha,(Hb,(Hc,Hd))))). clear Hd.
+  assert(Forall
+       (fun u : option gtt =>
+        u = None \/
+        (exists (g : gtt) (lsg : seq.seq (option (sort * gtt))),
+           u = Some g /\
+           g = gtt_send q p lsg)) ctxG).
+  {
+    apply Forall_forall; intros.
+    specialize(Forall_forall (fun u : option gtt =>
+        u = None \/
+        (exists (g : gtt) (lsg : seq.seq (option (sort * gtt))),
+           u = Some g /\
+           g = gtt_send q p lsg /\
+           Forall2
+             (fun (u0 : option (sort * gtt)) (v : option (sort * ltt)) =>
+              u0 = None /\ v = None \/
+              (exists (s : sort) (t : ltt) (g' : gtt),
+                 u0 = Some (s, g') /\ v = Some (s, t) /\ projectionC g' q t)) lsg LP)) ctxG); intros.
+    destruct H6. specialize(H6 Hc). clear Hc H7.
+    specialize(H6 x H5). destruct H6. left. easy.
+    destruct H6 as (g,(lsg,(Hc,(Hd,He)))). right. exists g. exists lsg. easy.
+  }
+  clear Hc.
+  revert H5 Hb Ha H4 H3 H2 H1 H0 H.
+  revert G G' p q pt l LP LQ ctxG.
+  induction Gl using gtth_ind_ref; intros.
+  - inversion Ha. subst.
+    specialize(some_onth_implies_In n ctxG G H8); intros.
+    specialize(Forall_forall (fun u : option gtt =>
+        u = None \/
+        (exists (g : gtt) (lsg : seq.seq (option (sort * gtt))), u = Some g /\ g = gtt_send q p lsg))
+       ctxG); intros.
+    destruct H7. specialize(H7 H5). clear H9 H5.
+    specialize(H7 (Some G) H6). destruct H7; try easy.
+    destruct H5 as (g1,(lsg,(Hc,Hd))). inversion Hc. subst.
+    pinversion H1; try easy. subst.
+    clear H11 H12.
+    unfold wfgC in H. destruct H. destruct H. rename x into G1.
+    unfold isgPartsC. destruct H5. destruct H7.
+    specialize(part_after_step_helper G1 q p lsg H H7); intros.
+    destruct H10. destruct H10.
+    specialize(part_after_step_helper2 l lsg q p x G' pt s); intros. apply H12; try easy.
+    apply step_mon.
+  - inversion Ha. subst.
+    unfold isgPartsC.
+    pinversion H2; try easy.
+    subst. assert False. apply Hb. constructor. easy.
+    subst. pinversion H3; try easy. subst.
+    pinversion H1; try easy. subst. clear H10 H11 H14 H16 H17 H20.
+    specialize(part_break (gtt_send p q ys2) pt H0 H4); intros.
+    destruct H7 as (Gl,(Hc,(Hd,(He,Hf)))).
+    destruct Hf.
+    - subst. pinversion Hc; try easy.
+    - destruct H7 as (p1,(q1,(lis1,Hf))). subst.
+      pinversion Hc; try easy. subst.
+    clear Hc.
+    - specialize(part_break (gtt_send p q ys) p); intros.
+      assert(exists Gl : global,
+       gttTC Gl (gtt_send p q ys) /\
+       isgParts p Gl /\
+       (forall n : fin, exists m : fin, guardG n m Gl) /\
+       (Gl = g_end \/
+        (exists (p q : string) (lis : seq.seq (option (sort * global))), Gl = g_send p q lis))).
+      {
+        apply H7; try easy.
+        apply triv_pt_p; try easy.
+      }
+      destruct H9 as (Gl1,(Hta,(Htb,(Htc,Htd)))).
+      destruct Htd. subst. pinversion Hta; try easy.
+      destruct H9 as (p1,(q1,(lsg1,Htd))). subst.
+      pinversion Hta. subst.
+    - rename p into st. rename q into st'. rename p0 into p. rename q0 into q.
+      clear H7 Hta.
+      inversion Hd; try easy. 
+      - subst. exists (g_send st st' lsg1). split. pfold. constructor. easy. split. easy. constructor.
+      - subst. exists (g_send st st' lsg1). split. pfold. constructor. easy. split. easy. constructor.
+      subst.
+      clear Htb H21 H15 H12 H4 H1 Ha H2 H3.
+      specialize(wfgC_after_step_all H23 H0); intros.
+      specialize(wfgC_after_step_all H23 H6); intros.
+      clear H0 H6 Hd H34.
+      specialize(part_after_step_helper3 n lis1 ys2 ys ys1 ys0 xs p q l s g ctxG); intros.
+      assert(exists (g' g'' : gtt) (t t' : ltt) (Gl : gtth),
+       onth n ys2 = Some (s, g') /\
+       gttTC g g' /\
+       onth n ys = Some (s, g'') /\
+       gttstepC g'' g' q p l /\
+       onth n ys1 = Some t /\
+       projectionC g'' q t /\
+       onth n ys0 = Some t' /\
+       projectionC g'' p t' /\ onth n xs = Some (s, Gl) /\ typ_gtth ctxG Gl g'').
+      {
+        apply H0; try easy.
+      }
+      clear H0.
+      destruct H3 as (g1,(g2,(t1,(t2,(Gl,(Hta,(Htb,(Htk,(Htd,(Hte,(Htf,(Hth,(Hti,(Htj,Htl)))))))))))))).
+      specialize(some_onth_implies_In n xs (s, Gl) Htj); intros.
+      specialize(Forall_forall (fun u : option (sort * gtth) =>
+       u = None \/
+       (exists (s : sort) (g : gtth),
+          u = Some (s, g) /\
+          (forall (G G' : gtt) (p q pt : string) (l : fin) (LP LQ : seq.seq (option (sort * ltt)))
+             (ctxG : seq.seq (option gtt)),
+           Forall
+             (fun u0 : option gtt =>
+              u0 = None \/
+              (exists (g0 : gtt) (lsg : seq.seq (option (sort * gtt))),
+                 u0 = Some g0 /\ g0 = gtt_send q p lsg)) ctxG ->
+           (ishParts q g -> False) ->
+           typ_gtth ctxG g G ->
+           isgPartsC pt G' ->
+           projectionC G q (ltt_send p LP) ->
+           projectionC G p (ltt_recv q LQ) ->
+           gttstepC G G' q p l -> wfgC G' -> wfgC G -> isgPartsC pt G))) xs); intros.
+      destruct H3. specialize(H3 H). clear H H4.
+      specialize(H3 (Some (s, Gl)) H0). destruct H3; try easy. 
+      destruct H as (s1,(g3,(Hma,Hmb))). inversion Hma. subst.
+      clear Hma H0.
+      specialize(Hmb g2 g1 p q pt l).
+      specialize(merge_onth_send n p LP ys1 t1 H25 Hte); intros. destruct H. subst.
+      specialize(merge_onth_recv n q LQ ys0 t2 H19 Hth); intros. destruct H. subst.
+      specialize(Hmb x x0 ctxG H5).
+      assert(isgPartsC pt g2).
+      {
+        apply Hmb; try easy.
+        specialize(ishParts_n Hb Htj); try easy.
+        unfold isgPartsC. exists g. split. easy. split; try easy.
+        specialize(guard_cont He); intros.
+        revert n0. specialize(Forall_prop n lis1 (s1, g) (fun u : option (sort * global) =>
+       u = None \/
+       (exists (s : sort) (g : global),
+          u = Some (s, g) /\ (forall n : fin, exists m : fin, guardG n m g))) H20 H); intro.
+        simpl in H0. destruct H0; try easy. destruct H0 as (st1,(gt1,(Hsa,Hsb))). inversion Hsa; try easy.
+        specialize(Forall_prop n ys2 (s1, g1) (fun u : option (sort * gtt) =>
+        u = None \/ (exists (st : sort) (g : gtt), u = Some (st, g) /\ wfgC g)) Hta H1); intro.
+        simpl in H. destruct H; try easy. destruct H as (st1,(gt1,(Hsa,Hsb))). inversion Hsa; try easy.
+        specialize(Forall_prop n ys (s1, g2) (fun u : option (sort * gtt) =>
+        u = None \/ (exists (st : sort) (g : gtt), u = Some (st, g) /\ wfgC g)) Htk H2); intro.
+        simpl in H. destruct H; try easy. destruct H as (st1,(gt1,(Hsa,Hsb))). inversion Hsa; try easy.
+      }
+      
+      clear Hmb H2 H1.
+      specialize(part_after_step_helper2 n ys st st'); intros.
+      specialize(H0 lsg1 g2 pt s1). apply H0; try easy. pfold. constructor. easy.
+    apply gttT_mon.
+    apply gttT_mon.
+    apply step_mon.
+    apply proj_mon.
+    apply proj_mon. 
+Qed.
+
+Theorem wfgCw_after_step : forall G G' p q n, wfgC G -> gttstepC G G' p q n -> wfgCw G'. 
+Proof.
+  intros. 
+  pose proof H as Ht. unfold wfgC in H.
+  destruct H as (Gl,(Ha,(Hb,(Hc,Hd)))).
+  specialize(wfgC_step_part G G' p q n Ht H0); intros.
+  specialize(balanced_to_tree G p Ht H); intros. clear Ht H.
+  destruct H1 as (Gt,(ctxG,(Hta,(Htb,(Htc,Htd))))).
+  clear Htd.
+  revert Htc Htb Hta H0 Hd Hc Hb Ha.
+  revert G G' p q n Gl ctxG.
+  induction Gt using gtth_ind_ref; intros; try easy.
+  - inversion Hta. subst.
+    specialize(Forall_forall (fun u : option gtt =>
+         u = None \/
+         (exists (q : string) (lsg : seq.seq (option (sort * gtt))),
+            u = Some (gtt_send p q lsg) \/
+            u = Some (gtt_send q p lsg) \/ u = Some gtt_end)) ctxG); intros.
+    destruct H. specialize(H Htc). clear H1 Htc.
+    specialize(some_onth_implies_In n ctxG G H2); intros.
+    specialize(H (Some G) H1). destruct H; try easy. destruct H as (r,(lsg,Hsa)). clear H1.
+    - destruct Hsa. inversion H. subst. 
+      pinversion H0; try easy. subst. clear H6 H.
+      specialize(guard_breakG_s2 (gtt_send p q lsg) Gl Hc Hb Ha); intros.
+      clear Ha Hb Hc. clear Gl. destruct H as (Gl,(Ha,(Hb,(Hc,He)))).
+      destruct Ha. subst. pinversion He. apply gttT_mon.
+      destruct H as (p1,(q1,(lis1,H))). subst. pinversion He; try easy. subst.
+      inversion Hc. subst.
+      specialize(balanced_cont Hd); intros.
+      specialize(guard_cont Hb); intros.
+      specialize(wfgC_after_step_helper n0 s G' lsg lis1); intros.
+      assert(exists G1 : global,
+       onth n0 lis1 = Some (s, G1) /\
+       gttTC G1 G' /\
+       wfG G1 /\ balancedG G' /\ (forall n : fin, exists m : fin, guardG n m G1)).
+      apply H4; try easy. clear H4. clear H3 H H7 H1.
+      destruct H8 as (G1,(Hsa,(Hsb,(Htc,(Htd,Hte))))). exists G1. easy.
+      apply gttT_mon.
+      apply step_mon.
+    - destruct H. inversion H. subst. pinversion H0; try easy. apply step_mon.
+    - inversion H. subst. pinversion H0; try easy. apply step_mon.
+  - inversion Hta. subst.
+    assert(wfgC (gtt_send p q ys)).
+    {
+      unfold wfgC. exists Gl. easy.
+    }
+    rename H1 into Ht.
+    pinversion H0; try easy.
+    - subst. assert False. apply Htb. constructor. easy.
+    subst. rename p into s. rename q into s'. rename p0 into p. rename q0 into q.
+    specialize(guard_breakG_s2 (gtt_send s s' ys) Gl Hc Hb Ha); intros. clear Ha Hb Hc. clear Gl.
+    destruct H1 as (Gl,(Ha,(Hb,(Hc,He)))). destruct Ha. subst. pinversion He; try easy. apply gttT_mon.
+    destruct H1 as (p1,(q1,(lis,H1))). subst. pinversion He; try easy. subst. inversion Hc. subst.
+    specialize(balanced_cont Hd); intros.
+    specialize(guard_cont Hb); intros.
+    assert(List.Forall (fun u => u = None \/ (exists s g, u = Some (s, g) /\ wfgCw g)) ys0).
+    {
+      clear H14 H13 Hb Hc He H16 H11 H10 H9 H8 H5 H4 H6 Hta H0 Hd.
+      apply Forall_forall; intros. 
+      destruct x.
+      - specialize(in_some_implies_onth p0 ys0 H0); intros. destruct H4 as (n0 ,H4). clear H0.
+        right. destruct p0. exists s0. exists g. split. easy.
+        clear Ht.
+        revert H4 H3 H1 H15 H2 H17 H7 Htc H Htb.
+        revert g s0 lis ys ys0 ctxG n p q xs s s'.
+        induction n0; intros.
+        - destruct ys0; try easy. destruct ys; try easy. destruct lis; try easy.
+          destruct xs; try easy.
+          inversion H3. subst. clear H3. inversion H1. subst. clear H1. inversion H15. subst. clear H15.
+          inversion H2. subst. clear H2. inversion H17. subst. clear H17. inversion H7. subst. clear H7.
+          inversion H. subst. clear H.
+          clear H8 H9 H10 H14 H15 H17 H7.
+          simpl in H4. subst.
+          destruct H11; try easy. destruct H as (s1,(g1,(g2,(Ha,(Hb,Hc))))). inversion Hb. subst.
+          destruct H13; try easy. destruct H as (s2,(g3,(g4,(Hd,(He,Hf))))). inversion He. subst.
+          destruct H12; try easy. destruct H as (s3,(g5,(g6,(Hg,(Hh,Hi))))). inversion Hh. subst.
+          destruct H3; try easy. destruct H as (s4,(g7,(Hj,Hk))). inversion Hj. subst.
+          destruct H6; try easy. destruct H as (s5,(g8,(Hl,Hm))). inversion Hl. subst.
+          destruct H5; try easy. destruct H as (s6,(g9,(Hn,Ho))). inversion Hn. subst.
+          destruct H2; try easy. clear Hn Hh He Hj Hl Hb.
+          destruct H as (s7,(g10,(Hp,Hq))). inversion Hp. subst.
+          specialize(Hq g9 g2 p q n g8 ctxG).
+          apply Hq; try easy. 
+          specialize(ishParts_x Htb); try easy.
+          destruct Hc; try easy.
+          destruct Hi; try easy. 
+        - destruct ys0; try easy. destruct ys; try easy. destruct lis; try easy.
+          destruct xs; try easy.
+          inversion H3. subst. clear H3. inversion H1. subst. clear H1. inversion H15. subst. clear H15.
+          inversion H2. subst. clear H2. inversion H17. subst. clear H17. inversion H7. subst. clear H7.
+          inversion H. subst. clear H. 
+          specialize(IHn0 g s0 lis ys ys0 ctxG n p q xs s s').
+          apply IHn0; try easy.
+          specialize(ishParts_hxs Htb); try easy.
+        left. easy.
+    }
+    specialize(wfgC_after_step_helper2 lis ys ys0 n p q H13 H2 H17); intros.
+    assert(wfgC (gtt_send s s' ys) /\ gttstepC (gtt_send s s' ys) (gtt_send s s' ys0) p q n). 
+    {
+      unfold wfgC. split. exists (g_send s s' lis). split. pfold. easy. easy.
+      pfold. easy.
+    }
+    destruct H19.
+    clear H3 H1 H15 H2 Hb Hc He H17 H16 H11 H10 H9 H8 H5 H4 H7 Hta H0 Hd Htb Htc H H6 H13. clear Ht H19 H20.
+    clear p q xs n ctxG ys lis. rename H14 into H. rename H12 into H1.
+    assert(exists xs, List.Forall2 (fun u v => (u = None /\ v = None) \/ (exists s g g', u = Some(s, g) /\ v = Some(s, g') /\ gttTC g g')) xs ys0 /\ 
+    List.Forall (fun u => u = None \/ (exists s g, u = Some(s, g) /\ wfG g)) xs /\
+    List.Forall (fun u => u = None \/ (exists s g, u = Some(s, g) /\ (forall n, exists m, guardG n m g))) xs).
+    {
+      clear H. revert H1. clear H18. revert ys0. clear s s'.
+      induction ys0; intros; try easy.
+      - exists nil. easy.
+      - inversion H1. subst. clear H1.
+        specialize(IHys0 H3). destruct IHys0 as (xs,H).
+        destruct H2. 
+        - subst. exists (None :: xs).
+          split. constructor; try easy. left. easy.
+          split. constructor; try easy. left. easy.
+          constructor; try easy. left. easy.
+        - destruct H0 as (s,(g,(Ha,Hb))). subst.
+          unfold wfgC in Hb. destruct Hb.
+          exists (Some(s, x) :: xs).
+          split. constructor; try easy. right. exists s. exists x. exists g. easy.
+          split. constructor; try easy. right. exists s. exists x. easy.
+          constructor; try easy. right. exists s. exists x. easy.
+    }
+    destruct H0 as (xs,(Ha,(Hb,Hc))).
+    exists (g_send s s' xs).
+    - split. pfold. constructor; try easy.
+      revert Ha. apply Forall2_mono; intros; try easy. destruct H0. left. easy.
+      destruct H0 as (s0,(g0,(g1,(Hta,(Htb,Htc))))). subst. right. exists s0. exists g0. exists g1. 
+      split. easy. split. easy. left. easy.
+    - split. constructor; try easy.
+      specialize(wfgC_after_step_helper3 ys0 xs H18 Ha); try easy.
+    - apply guard_cont_b; try easy.
+    apply gttT_mon.
+    apply step_mon.
+Qed.
+
+
